added manual proofs of multiple other small programs in suslik semantics

vst/listfree4.c
@@ -1,14 +1,22 @@
 #include <stddef.h>
 
+typedef union sslval {
+  int ssl_int;
+  void *ssl_ptr;
+} *loc;
+#define READ_LOC(x,y) (*(x+y)).ssl_ptr
+#define READ_INT(x,y) (*(x+y)).ssl_int
+
 extern void free(void *p);
 
-void listfree(void * x) {
+void listfree(loc x) {
   if((x == 0)) {
     return;
   } else {
-    void * n = *((void **)x + 1);
+    loc n = READ_LOC(x,1);
     listfree(n);
     free(x);
     return;
   }
 }
+
