vst/sumptr.c
@@ -10,9 +10,8 @@ typedef union sslval {
 #define WRITE_INT(x,y,z) (*(x+y)).ssl_int = z
 
 
-void swap(loc x, loc y) {
-  loc a2 = READ_LOC(x,0);
-  loc b2 = READ_LOC(y,0);
-  WRITE_LOC(y,0,a2);
-  WRITE_LOC(x,0,b2);
+void sumptr(loc x) {
+  int a2 = READ_INT(x,0);
+  int b2 = READ_INT(x,1);
+  WRITE_INT(x,2,a2 + b2);
 }
