vst/verif_min2.v
@@ -1,0 +1,59 @@
+Require Import VST.floyd.proofauto.
+
+Require Import min2.
+Instance CompSpecs : compspecs. make_compspecs prog. Defined.
+Definition Vprog : varspecs. mk_varspecs prog. Defined.
+
+Definition ssl_is_valid_int (x: val) := exists y, x = Vint (Int.repr y) /\  Int.min_signed <= y <= Int.max_signed.
+
+Ltac ssl_open_context :=
+  lazymatch goal with
+  | [ H:  ssl_is_valid_int ?x |- _ ] =>
+    let x1 := fresh x in
+    rename x into x1;
+    let H2 := fresh H in
+    let H3 := fresh H in
+    destruct H as [x [H2 H3]]; rewrite H2; ssl_open_context
+  | _ => idtac
+  end.
+
+
+Definition min2_spec :=
+  DECLARE _min2
+   WITH r: val, x: val, y: val
+   PRE [ (tptr (Tunion _sslval noattr)), tint, tint ]
+   PROP( is_pointer_or_null(r); ssl_is_valid_int(x); ssl_is_valid_int(y) )
+   PARAMS(r; x; y)
+   SEP ((data_at Tsh (tarray (Tunion _sslval noattr) 1) [inl (Vint (Int.repr 0))] r))
+   POST[ tvoid ]
+   EX m: Z,
+   PROP( (m <= (force_signed_int x)); (m <= (force_signed_int y)) )
+   LOCAL()
+   SEP ((data_at Tsh (tarray (Tunion _sslval noattr) 1) [inl (Vint (Int.repr m))] r)).
+
+
+
+(* Packaging the API spec all together. *)
+Definition Gprog : funspecs :=
+  ltac:(with_library prog [min2_spec]).
+
+From mathcomp Require Import ssreflect ssrbool.
+
+(** Proof that f_swap, the body of the swap() function,
+ ** satisfies swap_spec, in the global context (Vprog,Gprog).
+ **)
+Lemma min2_swap: semax_body Vprog Gprog f_min2 min2_spec.
+Proof.
+  start_function.
+  ssl_open_context.
+  forward_if.
+  - forward.
+    forward.
+    Exists x.
+    entailer.
+  - forward.
+    forward.
+    Exists y.
+    entailer!.
+Qed.
+
