vst/verif_sumptr.v
@@ -1,0 +1,39 @@
+Require Import VST.floyd.proofauto.
+
+Require Import sumptr.
+Instance CompSpecs : compspecs. make_compspecs prog. Defined.
+Definition Vprog : varspecs. mk_varspecs prog. Defined.
+
+
+Definition sumptr_spec : ident * funspec :=
+  DECLARE _sumptr
+   WITH x: val, a: Z, b: Z
+   PRE  [(tptr (Tunion _sslval noattr))]
+   PROP (a + b < Int.max_signed)
+   PARAMS(x)
+   SEP  (data_at Tsh (tarray (Tunion _sslval noattr) 3)
+                 [(inl (Vint (Int.repr a))); (inl (Vint (Int.repr b))); (inl (Vint (Int.repr 0)))] x)
+   POST [tvoid]
+         PROP ()
+         LOCAL()
+         SEP
+         (data_at Tsh (tarray (Tunion _sslval noattr) 3)
+                 [(inl (Vint (Int.repr a))); (inl (Vint (Int.repr b))); (inl (Vint (Int.repr (a + b))))] x).
+
+(* Packaging the API spec all together. *)
+Definition Gprog : funspecs :=
+  ltac:(with_library prog [sumptr_spec]).
+
+(** Proof that f_swap, the body of the swap() function,
+ ** satisfies swap_spec, in the global context (Vprog,Gprog).
+ **)
+Lemma body_sumptr: semax_body Vprog Gprog f_sumptr sumptr_spec.
+Proof.
+  start_function.
+  forward.
+  forward.
+  forward.
+  entailer!.
+  admit.
+  entailer!.
+Qed.
